<?xml version="1.0"?>
<rdf:RDF xmlns="http://purl.obolibrary.org/obo/opmi/IAO_imports.owl#"
     xml:base="http://purl.obolibrary.org/obo/opmi/IAO_imports.owl"
     xmlns:obo="http://purl.obolibrary.org/obo/"
     xmlns:rdfs="http://www.w3.org/2000/01/rdf-schema#"
     xmlns:owl="http://www.w3.org/2002/07/owl#"
     xmlns:xsd="http://www.w3.org/2001/XMLSchema#"
     xmlns:rdf="http://www.w3.org/1999/02/22-rdf-syntax-ns#">
    <owl:Ontology rdf:about="http://purl.obolibrary.org/obo/opmi/IAO_imports.owl"/>
    


    <!-- 
    ///////////////////////////////////////////////////////////////////////////////////////
    //
    // Annotation properties
    //
    ///////////////////////////////////////////////////////////////////////////////////////
     -->

    <owl:AnnotationProperty rdf:about="http://purl.obolibrary.org/obo/IAO_0000115">
        <rdfs:label rdf:datatype="http://www.w3.org/2001/XMLSchema#string">definition</rdfs:label>
        <rdfs:label xml:lang="en">definition</rdfs:label>
        <obo:IAO_0000115 xml:lang="en">The official definition, explaining the meaning of a class or property. Shall be Aristotelian, formalized and normalized. Can be augmented with colloquial definitions.</obo:IAO_0000115>
    </owl:AnnotationProperty>
    <owl:AnnotationProperty rdf:about="http://purl.obolibrary.org/obo/IAO_0000412">
        <rdfs:label xml:lang="en">imported from</rdfs:label>
    </owl:AnnotationProperty>
    <owl:AnnotationProperty rdf:about="http://www.w3.org/2000/01/rdf-schema#label"/>
    


    <!-- 
    ///////////////////////////////////////////////////////////////////////////////////////
    //
    // Datatypes
    //
    ///////////////////////////////////////////////////////////////////////////////////////
     -->

    


    <!-- 
    ///////////////////////////////////////////////////////////////////////////////////////
    //
    // Object Properties
    //
    ///////////////////////////////////////////////////////////////////////////////////////
     -->

    


    <!-- http://purl.obolibrary.org/obo/IAO_0000136 -->

    <owl:ObjectProperty rdf:about="http://purl.obolibrary.org/obo/IAO_0000136">
        <rdfs:label xml:lang="en">is about</rdfs:label>
        <obo:IAO_0000115 xml:lang="en">is_about is a (currently) primitive relation that relates an information artifact to an entity.</obo:IAO_0000115>
        <obo:IAO_0000412 rdf:resource="http://purl.obolibrary.org/obo/iao.owl"/>
    </owl:ObjectProperty>
    


    <!-- http://purl.obolibrary.org/obo/IAO_0000413 -->

    <owl:ObjectProperty rdf:about="http://purl.obolibrary.org/obo/IAO_0000413">
        <rdfs:label xml:lang="en">is duration of</rdfs:label>
        <obo:IAO_0000115 xml:lang="en">relates a process to a time-measurement-datum that represents the duration of the process</obo:IAO_0000115>
        <rdfs:subPropertyOf rdf:resource="http://purl.obolibrary.org/obo/IAO_0000136"/>
        <obo:IAO_0000412 rdf:resource="http://purl.obolibrary.org/obo/iao.owl"/>
    </owl:ObjectProperty>
    


    <!-- 
    ///////////////////////////////////////////////////////////////////////////////////////
    //
    // Classes
    //
    ///////////////////////////////////////////////////////////////////////////////////////
     -->

    


    <!-- http://purl.obolibrary.org/obo/IAO_0000017 -->

    <owl:Class rdf:about="http://purl.obolibrary.org/obo/IAO_0000017">
        <rdfs:label xml:lang="en">model number</rdfs:label>
        <rdfs:subClassOf rdf:resource="http://purl.obolibrary.org/obo/IAO_0000028"/>
        <obo:IAO_0000115 xml:lang="en">A model number is an information content entity specifically borne by catalogs, design specifications, advertising materials, inventory systems and similar  that is about manufactured objects of the same class. The model number is an alternative term for the class. The manufactered objects may or may not also bear the model number. Model numbers can be encoded in a variety of other information objects, such as bar codes, numerals, or patterns of dots.</obo:IAO_0000115>
        <obo:IAO_0000412 rdf:resource="http://purl.obolibrary.org/obo/iao.owl"/>
    </owl:Class>
    


    <!-- http://purl.obolibrary.org/obo/IAO_0000027 -->

    <owl:Class rdf:about="http://purl.obolibrary.org/obo/IAO_0000027">
        <rdfs:label xml:lang="en">data item</rdfs:label>
        <rdfs:subClassOf rdf:resource="http://purl.obolibrary.org/obo/IAO_0000030"/>
        <obo:IAO_0000115 xml:lang="en">a data item is an information content entity that is intended to be a truthful statement about something (modulo, e.g., measurement precision or other systematic errors) and is constructed/acquired by a method which reliably tends to produce (approximately) truthful statements.</obo:IAO_0000115>
        <obo:IAO_0000412 rdf:resource="http://purl.obolibrary.org/obo/iao.owl"/>
    </owl:Class>
    


    <!-- http://purl.obolibrary.org/obo/IAO_0000028 -->

    <owl:Class rdf:about="http://purl.obolibrary.org/obo/IAO_0000028">
        <rdfs:label xml:lang="en">symbol</rdfs:label>
        <rdfs:subClassOf rdf:resource="http://purl.obolibrary.org/obo/IAO_0000030"/>
        <obo:IAO_0000115 xml:lang="en">An information content entity that is a mark(s) or character(s) used as a conventional representation of another entity.</obo:IAO_0000115>
        <obo:IAO_0000412 rdf:resource="http://purl.obolibrary.org/obo/iao.owl"/>
    </owl:Class>
    


    <!-- http://purl.obolibrary.org/obo/IAO_0000029 -->

    <owl:Class rdf:about="http://purl.obolibrary.org/obo/IAO_0000029">
        <rdfs:label xml:lang="en">numeral</rdfs:label>
        <rdfs:subClassOf rdf:resource="http://purl.obolibrary.org/obo/IAO_0000028"/>
        <obo:IAO_0000115 xml:lang="en">A symbol that denotes a number.</obo:IAO_0000115>
        <obo:IAO_0000412 rdf:resource="http://purl.obolibrary.org/obo/iao.owl"/>
    </owl:Class>
    


    <!-- http://purl.obolibrary.org/obo/IAO_0000030 -->

    <owl:Class rdf:about="http://purl.obolibrary.org/obo/IAO_0000030">
        <rdfs:label xml:lang="en">information content entity</rdfs:label>
        <rdfs:subClassOf rdf:resource="http://purl.obolibrary.org/obo/IAO_0000030"/>
        <obo:IAO_0000115 xml:lang="en">A generically dependent continuant that is about some thing.</obo:IAO_0000115>
        <obo:IAO_0000412 rdf:resource="http://purl.obolibrary.org/obo/iao.owl"/>
    </owl:Class>
    


    <!-- http://purl.obolibrary.org/obo/IAO_0000031 -->

    <owl:Class rdf:about="http://purl.obolibrary.org/obo/IAO_0000031">
        <rdfs:label xml:lang="en">integer numeral</rdfs:label>
        <rdfs:subClassOf rdf:resource="http://purl.obolibrary.org/obo/IAO_0000029"/>
        <obo:IAO_0000115 xml:lang="en">a numeral that denotes an integer</obo:IAO_0000115>
        <obo:IAO_0000412 rdf:resource="http://purl.obolibrary.org/obo/iao.owl"/>
    </owl:Class>
    


    <!-- http://purl.obolibrary.org/obo/IAO_0000037 -->

    <owl:Class rdf:about="http://purl.obolibrary.org/obo/IAO_0000037">
        <rdfs:label xml:lang="en">dot plot</rdfs:label>
        <rdfs:subClassOf rdf:resource="http://purl.obolibrary.org/obo/IAO_0000038"/>
        <obo:IAO_0000115 xml:lang="en">A dot plot is a report graph which is a graphical representation of data where each data point is represented by a single dot placed on coordinates corresponding to data point values in particular dimensions.</obo:IAO_0000115>
        <obo:IAO_0000412 rdf:resource="http://purl.obolibrary.org/obo/iao.owl"/>
    </owl:Class>
    


    <!-- http://purl.obolibrary.org/obo/IAO_0000038 -->

    <owl:Class rdf:about="http://purl.obolibrary.org/obo/IAO_0000038">
        <rdfs:label xml:lang="en">graph</rdfs:label>
        <rdfs:subClassOf rdf:resource="http://purl.obolibrary.org/obo/IAO_0000309"/>
        <obo:IAO_0000115 xml:lang="en">A diagram that presents one or more tuples of information by mapping those tuples in to a two dimensional space in a non arbitrary way.</obo:IAO_0000115>
        <obo:IAO_0000412 rdf:resource="http://purl.obolibrary.org/obo/iao.owl"/>
    </owl:Class>
    


    <!-- http://purl.obolibrary.org/obo/IAO_0000057 -->

    <owl:Class rdf:about="http://purl.obolibrary.org/obo/IAO_0000057">
        <rdfs:label xml:lang="en">contour plot</rdfs:label>
        <rdfs:subClassOf rdf:resource="http://purl.obolibrary.org/obo/IAO_0000038"/>
        <obo:IAO_0000412 rdf:resource="http://purl.obolibrary.org/obo/iao.owl"/>
    </owl:Class>
    


    <!-- http://purl.obolibrary.org/obo/IAO_0000079 -->

    <owl:Class rdf:about="http://purl.obolibrary.org/obo/IAO_0000079">
        <rdfs:label xml:lang="en">density plot</rdfs:label>
        <rdfs:subClassOf rdf:resource="http://purl.obolibrary.org/obo/IAO_0000038"/>
        <obo:IAO_0000115 xml:lang="en">A density plot is a report graph which is a graphical representation of data where the tint of a particular pixel corresponds to some kind of function corresponding the the amount of data points relativelly with their distance from the the pixel.</obo:IAO_0000115>
        <obo:IAO_0000412 rdf:resource="http://purl.obolibrary.org/obo/iao.owl"/>
    </owl:Class>
    


    <!-- http://purl.obolibrary.org/obo/IAO_0000101 -->

    <owl:Class rdf:about="http://purl.obolibrary.org/obo/IAO_0000101">
        <rdfs:label xml:lang="en">image</rdfs:label>
        <rdfs:subClassOf rdf:resource="http://purl.obolibrary.org/obo/IAO_0000308"/>
        <obo:IAO_0000115 xml:lang="en">An image is an affine projection to a two dimensional surface, of measurements of some quality of an entity or entities repeated at regular intervals across a spatial range, where the measurements are represented as color and luminosity on the projected on surface.</obo:IAO_0000115>
        <obo:IAO_0000412 rdf:resource="http://purl.obolibrary.org/obo/iao.owl"/>
    </owl:Class>
    


    <!-- http://purl.obolibrary.org/obo/IAO_0000109 -->

    <owl:Class rdf:about="http://purl.obolibrary.org/obo/IAO_0000109">
        <rdfs:label xml:lang="en">measurement datum</rdfs:label>
        <rdfs:subClassOf rdf:resource="http://purl.obolibrary.org/obo/IAO_0000027"/>
        <obo:IAO_0000115 xml:lang="en">A measurement datum is an information content entity that is a recording of the output of a measurement such as produced by a device.</obo:IAO_0000115>
        <obo:IAO_0000412 rdf:resource="http://purl.obolibrary.org/obo/iao.owl"/>
    </owl:Class>
    


    <!-- http://purl.obolibrary.org/obo/IAO_0000129 -->

    <owl:Class rdf:about="http://purl.obolibrary.org/obo/IAO_0000129">
        <rdfs:label xml:lang="en">version number</rdfs:label>
        <rdfs:subClassOf rdf:resource="http://purl.obolibrary.org/obo/IAO_0000028"/>
        <obo:IAO_0000115 xml:lang="en">A version number is an information content entity which is a sequence of characters borne by part of each of a class of manufactured products or its packaging and indicates its order within a set of other products having the same name.</obo:IAO_0000115>
        <obo:IAO_0000412 rdf:resource="http://purl.obolibrary.org/obo/iao.owl"/>
    </owl:Class>
    


    <!-- http://purl.obolibrary.org/obo/IAO_0000131 -->

    <owl:Class rdf:about="http://purl.obolibrary.org/obo/IAO_0000131">
        <rdfs:label xml:lang="en">serial number</rdfs:label>
        <rdfs:subClassOf rdf:resource="http://purl.obolibrary.org/obo/IAO_0000028"/>
        <obo:IAO_0000115 xml:lang="en">A serial number is an information content entity which is a unique sequence of characters borne by part of manufactured product or its packaging that is assigned to each individual in some class of products, and so can serve as a way to identify an individual product within the class. Serial numbers can be encoded in a variety of other information objects, such as bar codes, numerals, or patterns of dots.</obo:IAO_0000115>
        <obo:IAO_0000412 rdf:resource="http://purl.obolibrary.org/obo/iao.owl"/>
    </owl:Class>
    


    <!-- http://purl.obolibrary.org/obo/IAO_0000132 -->

    <owl:Class rdf:about="http://purl.obolibrary.org/obo/IAO_0000132">
        <rdfs:label xml:lang="en">lot number</rdfs:label>
        <rdfs:subClassOf rdf:resource="http://purl.obolibrary.org/obo/IAO_0000028"/>
        <obo:IAO_0000115 xml:lang="en">A lot number is an information content entity which is an identical sequence of character borne by part of manufactured product or its packaging for each instances of a product class in a discrete batch of an item. Lot numbers are usually assigned to each separate production run of an item. Manufacturing as a lot might be due to a variety of reasons, for example,  a single process during which many individuals are made from the same portion of source material. Lot numbers can be encoded in a pattern  of other information objects, such as bar codes, numerals, or patterns of dots.</obo:IAO_0000115>
        <obo:IAO_0000412 rdf:resource="http://purl.obolibrary.org/obo/iao.owl"/>
    </owl:Class>
    


    <!-- http://purl.obolibrary.org/obo/IAO_0000179 -->

    <owl:Class rdf:about="http://purl.obolibrary.org/obo/IAO_0000179">
        <rdfs:label xml:lang="en">histogram</rdfs:label>
        <rdfs:subClassOf rdf:resource="http://purl.obolibrary.org/obo/IAO_0000038"/>
        <obo:IAO_0000115 xml:lang="en">A histogram is a report graph which is a statistical description of a
distribution in terms of occurrence frequencies of different event classes.</obo:IAO_0000115>
        <obo:IAO_0000412 rdf:resource="http://purl.obolibrary.org/obo/iao.owl"/>
    </owl:Class>
    


    <!-- http://purl.obolibrary.org/obo/IAO_0000180 -->

    <owl:Class rdf:about="http://purl.obolibrary.org/obo/IAO_0000180">
        <rdfs:label xml:lang="en">heatmap</rdfs:label>
        <rdfs:subClassOf rdf:resource="http://purl.obolibrary.org/obo/IAO_0000038"/>
        <obo:IAO_0000115 xml:lang="en">A heatmap is a report graph which is a graphical representation of data
where the values taken by a variable(s) are shown as colors in a
two-dimensional map.</obo:IAO_0000115>
        <obo:IAO_0000412 rdf:resource="http://purl.obolibrary.org/obo/iao.owl"/>
    </owl:Class>
    


    <!-- http://purl.obolibrary.org/obo/IAO_0000181 -->

    <owl:Class rdf:about="http://purl.obolibrary.org/obo/IAO_0000181">
        <rdfs:label xml:lang="en">Venn diagram</rdfs:label>
        <rdfs:subClassOf rdf:resource="http://purl.obolibrary.org/obo/IAO_0000038"/>
        <obo:IAO_0000115 xml:lang="en">A Venn diagram is a report graph showing all hypothetically possible
logical relations between a finite collection of sets.</obo:IAO_0000115>
        <obo:IAO_0000412 rdf:resource="http://purl.obolibrary.org/obo/iao.owl"/>
    </owl:Class>
    


    <!-- http://purl.obolibrary.org/obo/IAO_0000183 -->

    <owl:Class rdf:about="http://purl.obolibrary.org/obo/IAO_0000183">
        <rdfs:label xml:lang="en">dendrogram</rdfs:label>
        <rdfs:subClassOf rdf:resource="http://purl.obolibrary.org/obo/IAO_0000038"/>
        <obo:IAO_0000115 xml:lang="en">A dendrogram is a report graph which is a tree diagram
frequently used to illustrate the arrangement of the clusters produced by a
clustering algorithm.</obo:IAO_0000115>
        <obo:IAO_0000412 rdf:resource="http://purl.obolibrary.org/obo/iao.owl"/>
    </owl:Class>
    


    <!-- http://purl.obolibrary.org/obo/IAO_0000184 -->

    <owl:Class rdf:about="http://purl.obolibrary.org/obo/IAO_0000184">
        <rdfs:label xml:lang="en">scatter plot</rdfs:label>
        <rdfs:subClassOf rdf:resource="http://purl.obolibrary.org/obo/IAO_0000038"/>
        <obo:IAO_0000115 xml:lang="en">A scatterplot is a graph which uses Cartesian coordinates to display values for two variables for a set of data. The data is displayed as a collection of points, each having the value of one variable determining the position on the horizontal axis and the value of the other variable determining the position on the vertical axis.</obo:IAO_0000115>
        <obo:IAO_0000412 rdf:resource="http://purl.obolibrary.org/obo/iao.owl"/>
    </owl:Class>
    


    <!-- http://purl.obolibrary.org/obo/IAO_0000185 -->

    <owl:Class rdf:about="http://purl.obolibrary.org/obo/IAO_0000185">
        <rdfs:label xml:lang="en">photograph</rdfs:label>
        <rdfs:subClassOf rdf:resource="http://purl.obolibrary.org/obo/IAO_0000101"/>
        <obo:IAO_0000115 xml:lang="en">A photograph is created by projecting an image onto a photosensitive surface such as a chemically treated plate or film, CCD receptor, etc.</obo:IAO_0000115>
        <obo:IAO_0000412 rdf:resource="http://purl.obolibrary.org/obo/iao.owl"/>
    </owl:Class>
    


    <!-- http://purl.obolibrary.org/obo/IAO_0000300 -->

    <owl:Class rdf:about="http://purl.obolibrary.org/obo/IAO_0000300">
        <rdfs:label xml:lang="en">textual entity</rdfs:label>
        <rdfs:subClassOf rdf:resource="http://purl.obolibrary.org/obo/IAO_0000030"/>
        <obo:IAO_0000115 xml:lang="en">A textual entity is a part of a manifestation (FRBR sense), a generically dependent continuant whose concretizations are patterns of glyphs intended to be interpreted as words, formulas, etc.</obo:IAO_0000115>
        <obo:IAO_0000412 rdf:resource="http://purl.obolibrary.org/obo/iao.owl"/>
    </owl:Class>
    


    <!-- http://purl.obolibrary.org/obo/IAO_0000301 -->

    <owl:Class rdf:about="http://purl.obolibrary.org/obo/IAO_0000301">
        <rdfs:label xml:lang="en">citation</rdfs:label>
        <rdfs:subClassOf rdf:resource="http://purl.obolibrary.org/obo/IAO_0000300"/>
        <obo:IAO_0000115 xml:lang="en">a textual entity intended to identify a particular publication</obo:IAO_0000115>
        <obo:IAO_0000412 rdf:resource="http://purl.obolibrary.org/obo/iao.owl"/>
    </owl:Class>
    


    <!-- http://purl.obolibrary.org/obo/IAO_0000305 -->

    <owl:Class rdf:about="http://purl.obolibrary.org/obo/IAO_0000305">
        <rdfs:label xml:lang="en">document title</rdfs:label>
        <rdfs:subClassOf rdf:resource="http://purl.obolibrary.org/obo/IAO_0000300"/>
        <obo:IAO_0000115 xml:lang="en">A textual entity that names a document</obo:IAO_0000115>
        <obo:IAO_0000412 rdf:resource="http://purl.obolibrary.org/obo/iao.owl"/>
    </owl:Class>
    


    <!-- http://purl.obolibrary.org/obo/IAO_0000306 -->

    <owl:Class rdf:about="http://purl.obolibrary.org/obo/IAO_0000306">
        <rdfs:label xml:lang="en">table</rdfs:label>
        <rdfs:subClassOf rdf:resource="http://purl.obolibrary.org/obo/IAO_0000300"/>
        <obo:IAO_0000115 xml:lang="en">A textual entity that contains a two-dimensional arrangement of texts repeated at regular intervals across a spatial range, such that the spatial relationships among the constituent texts expresses propositions</obo:IAO_0000115>
        <obo:IAO_0000412 rdf:resource="http://purl.obolibrary.org/obo/iao.owl"/>
    </owl:Class>
    


    <!-- http://purl.obolibrary.org/obo/IAO_0000308 -->

    <owl:Class rdf:about="http://purl.obolibrary.org/obo/IAO_0000308">
        <rdfs:label xml:lang="en">figure</rdfs:label>
        <rdfs:subClassOf rdf:resource="http://purl.obolibrary.org/obo/IAO_0000030"/>
        <obo:IAO_0000115 xml:lang="en">An information content entity consisting of a two dimensional arrangement of information content entities such that the arrangement itself is about something.</obo:IAO_0000115>
        <obo:IAO_0000412 rdf:resource="http://purl.obolibrary.org/obo/iao.owl"/>
    </owl:Class>
    


    <!-- http://purl.obolibrary.org/obo/IAO_0000309 -->

    <owl:Class rdf:about="http://purl.obolibrary.org/obo/IAO_0000309">
        <rdfs:label xml:lang="en">diagram</rdfs:label>
        <rdfs:subClassOf rdf:resource="http://purl.obolibrary.org/obo/IAO_0000308"/>
        <obo:IAO_0000115 xml:lang="en">A figure that expresses one or more propositions</obo:IAO_0000115>
        <obo:IAO_0000412 rdf:resource="http://purl.obolibrary.org/obo/iao.owl"/>
    </owl:Class>
    


    <!-- http://purl.obolibrary.org/obo/IAO_0000415 -->

    <owl:Class rdf:about="http://purl.obolibrary.org/obo/IAO_0000415">
        <rdfs:label xml:lang="en">hypothesis textual entity</rdfs:label>
        <rdfs:subClassOf rdf:resource="http://purl.obolibrary.org/obo/IAO_0000300"/>
        <obo:IAO_0000115 xml:lang="en">A textual entity that expresses an assertion that is intended to be tested.</obo:IAO_0000115>
        <obo:IAO_0000412 rdf:resource="http://purl.obolibrary.org/obo/iao.owl"/>
    </owl:Class>
    


    <!-- http://purl.obolibrary.org/obo/IAO_0000422 -->

    <owl:Class rdf:about="http://purl.obolibrary.org/obo/IAO_0000422">
        <rdfs:label xml:lang="en">postal address</rdfs:label>
        <rdfs:subClassOf rdf:resource="http://purl.obolibrary.org/obo/IAO_0000300"/>
        <obo:IAO_0000115>A textual entity that is used as directive to deliver something to a person, or organization</obo:IAO_0000115>
        <obo:IAO_0000412 rdf:resource="http://purl.obolibrary.org/obo/iao.owl"/>
    </owl:Class>
    


    <!-- http://purl.obolibrary.org/obo/IAO_0000429 -->

    <owl:Class rdf:about="http://purl.obolibrary.org/obo/IAO_0000429">
        <rdfs:label xml:lang="en">email address</rdfs:label>
        <rdfs:subClassOf rdf:resource="http://purl.obolibrary.org/obo/IAO_0000030"/>
        <obo:IAO_0000412 rdf:resource="http://purl.obolibrary.org/obo/iao.owl"/>
    </owl:Class>
    


    <!-- http://purl.obolibrary.org/obo/IAO_0000573 -->

    <owl:Class rdf:about="http://purl.obolibrary.org/obo/IAO_0000573">
        <rdfs:label xml:lang="en">line graph</rdfs:label>
        <rdfs:subClassOf rdf:resource="http://purl.obolibrary.org/obo/IAO_0000038"/>
        <obo:IAO_0000115 xml:lang="en">A line graph is a type of graph created by connecting a series of data
points together with a line.</obo:IAO_0000115>
        <obo:IAO_0000412 rdf:resource="http://purl.obolibrary.org/obo/iao.owl"/>
    </owl:Class>
    


    <!-- http://purl.obolibrary.org/obo/IAO_0000577 -->

    <owl:Class rdf:about="http://purl.obolibrary.org/obo/IAO_0000577">
        <rdfs:label xml:lang="en">centrally registered identifier symbol</rdfs:label>
        <rdfs:subClassOf rdf:resource="http://purl.obolibrary.org/obo/IAO_0000028"/>
        <obo:IAO_0000115 xml:lang="en">A symbol that is part of a CRID and that is sufficient to look up a record from the CRID&#39;s registry.</obo:IAO_0000115>
        <obo:IAO_0000412 rdf:resource="http://purl.obolibrary.org/obo/iao.owl"/>
    </owl:Class>
    


    <!-- http://purl.obolibrary.org/obo/IAO_0000590 -->

    <owl:Class rdf:about="http://purl.obolibrary.org/obo/IAO_0000590">
        <rdfs:label xml:lang="en">written name</rdfs:label>
        <rdfs:subClassOf rdf:resource="http://purl.obolibrary.org/obo/IAO_0000300"/>
        <obo:IAO_0000115 xml:lang="en">A textual entity that denotes a particular in reality.</obo:IAO_0000115>
        <obo:IAO_0000412 rdf:resource="http://purl.obolibrary.org/obo/iao.owl"/>
    </owl:Class>
    


    <!-- http://purl.obolibrary.org/obo/IAO_0000608 -->

    <owl:Class rdf:about="http://purl.obolibrary.org/obo/IAO_0000608">
        <rdfs:label xml:lang="en">author information textual entity</rdfs:label>
        <rdfs:subClassOf rdf:resource="http://purl.obolibrary.org/obo/IAO_0000300"/>
        <obo:IAO_0000115 xml:lang="en">A textual entity expression information about an author of a document. This information may include biographical information and may discuss how the authors&#39; professional experiences are relevant to the work described in the document.</obo:IAO_0000115>
        <obo:IAO_0000412 rdf:resource="http://purl.obolibrary.org/obo/iao.owl"/>
    </owl:Class>
    


    <!-- http://purl.obolibrary.org/obo/IAO_0000614 -->

    <owl:Class rdf:about="http://purl.obolibrary.org/obo/IAO_0000614">
        <rdfs:label xml:lang="en">case report textual entity</rdfs:label>
        <rdfs:subClassOf rdf:resource="http://purl.obolibrary.org/obo/IAO_0000300"/>
        <obo:IAO_0000115 xml:lang="en">A textual entity that expresses a detailed account of a portion of the medical history for a specific patient.</obo:IAO_0000115>
        <obo:IAO_0000412 rdf:resource="http://purl.obolibrary.org/obo/iao.owl"/>
    </owl:Class>
</rdf:RDF>



<!-- Generated by the OWL API (version 3.2.4.1806) http://owlapi.sourceforge.net -->

